Move most things over into Slice/Basic.lean

LeanSorting/Slice/Basic.lean
@@ -1,4 +1,20 @@
 import Mathlib.Data.Nat.Defs
+import Batteries.Classes.Order
+import LeanSorting.Nat.Extras
+
+open Batteries
+
+variable
+  {α : Type}
+  [Ord α]
+  [LE α]
+  [LT α]
+  [BEq α]
+  [LawfulOrd α]
+  {arr arr₁ arr₂ arr_i aux : Array α}
+  {low high low₁ high₁ low₂ high₂ ptr ptr₁ ptr₂ mid : ℕ}
+  (s : @Slice α arr low high)
+  (s_i : @Slice α arr_i low_i high_i)
 
 structure Slice (arr : Array α) (low high : ℕ) : Prop where
   low_le_high : low ≤ high
@@ -69,3 +85,223 @@ def SlicePtrInclusive.make_exclusive
     (ptr_lt_high : ptr < high)
     : SlicePtrExclusive arr low high ptr :=
   { s with ptr_lt_high }
+
+-- TODO: must also be a permutation of input
+def Slice.sorted (_s : Slice arr low high) : Prop :=
+  ∀ (i₁ i₂ : Fin arr.size)
+    (_adjacent_in_range : i₁.val.adjacent_in_range i₂ low high),
+      Ord.compare arr[i₁] arr[i₂] ≠ Ordering.gt
+
+/--
+A slice s₁ is less than or equal to a slice s₂ if every element of s₁
+is less than or equal to every element of s₂.
+-/
+def Slice.le
+    (_s₁ : Slice arr₁ low₁ high₁)
+    (_s₂ : Slice arr₂ low₂ high₂)
+    : Prop :=
+  ∀ (i₁ : Fin arr₁.size) (i₂ : Fin arr₂.size),
+      i₁.val.in_range low₁ high₁
+    ∧ i₂.val.in_range low₂ high₂
+    → Ord.compare arr₁[i₁] arr₂[i₂] ≠ Ordering.gt
+
+/--
+A `Slice` `s₁` is less than or equal to an element `a` if every element of
+`s₁` is less than or equal to `a`.
+-/
+def Slice.le_elem (s : Slice arr low high) (a : α) : Prop :=
+  ∀ (i : ℕ) (in_bounds : i ≥ low ∧ i < high),
+    have high_le_size := s.high_le_size
+    Ord.compare arr[i] a ≠ Ordering.gt
+
+/--
+A `Slice` `s₁` is greater than or equal to an element `a` if every element of
+`s₁` is greater than or equal to `a`.
+-/
+def Slice.ge_elem (s : Slice arr low high) (a : α) :=
+  ∀ (i : ℕ) (in_bounds : i ≥ low ∧ i < high),
+    have high_le_size := s.high_le_size
+    Ord.compare a arr[i] ≠ Ordering.gt
+
+/--
+For slices `s₁` and `s₂`, `s₁.le s₂` implies `s₁.le_elem a`, where `a` is any
+element of `s₂`.
+-/
+def Slice.le_elem_of_le
+    (s₁ : Slice arr₁ low₁ high₁)
+    {s₂ : Slice arr₂ low₂ high₂}
+    (s₁_le_s₂ : s₁.le s₂)
+    (ptr_in_bounds₂ : ptr ≥ low₂ ∧ ptr < high₂)
+    : have high_le_size := s₂.high_le_size
+      s₁.le_elem arr₂[ptr] := by
+  intro high_le_size
+  unfold Slice.le_elem
+  intro i in_bounds high_le_size
+  unfold Slice.le at s₁_le_s₂
+  have i_lt_arr₁_size : i < arr₁.size := by omega
+  have ptr_lt_arr₂_size : ptr < arr₂.size := by omega
+  have h : i.in_range low₁ high₁ ∧ ptr.in_range low₂ high₂ := by
+    simp [Nat.in_range]
+    omega
+  exact s₁_le_s₂ ⟨i, i_lt_arr₁_size⟩ ⟨ptr, ptr_lt_arr₂_size⟩ h
+
+lemma not_gt_of_compare_same {a : α} : compare a a ≠ Ordering.gt := by
+  have compare_refl : compare a a = .eq := by exact Batteries.OrientedCmp.cmp_refl
+  intro compare_eq_gt
+  have : Ordering.eq = Ordering.gt := by rw [← compare_refl, ← compare_eq_gt]
+  contradiction
+
+/--
+If a Slice `s` is sorted and `a` is its first element, then `s.ge_elem a` is true.
+-/
+def Slice.ge_elem_low_of_sorted
+    (s_sorted : s.sorted)
+    (nonempty : low < high)
+    : have := s.high_le_size
+      s.ge_elem arr[low]
+    := by
+  simp [Slice.ge_elem]
+  intro i in_bounds
+  simp [Slice.sorted] at s_sorted
+  have := s.low_le_high
+  have := s.high_le_size
+  let rec loop (i : ℕ) (in_bounds : i ≥ low ∧ i < high)
+      : compare arr[low] arr[i] ≠ Ordering.gt := by
+    if i_eq_low : i = low then
+      simp [i_eq_low]
+      exact not_gt_of_compare_same
+    else
+      let j := i - 1
+      have j_in_bounds : j ≥ low ∧ j < high := by omega
+      have ih := loop j j_in_bounds
+      let j_f : Fin arr.size := ⟨j, by omega⟩
+      let i_f : Fin arr.size := ⟨i, by omega⟩
+      have adj : j_f.val.adjacent_in_range i_f low high := by
+        simp [Nat.adjacent_in_range]
+        omega
+      have h := s_sorted j_f i_f adj
+      exact TransCmp.le_trans ih h
+  exact loop i in_bounds
+
+def Slice.ge_elem_low_succ_of_sorted
+    (s_sorted : s.sorted)
+    (nonempty : low < high)
+    (s' : Slice arr low.succ high)
+    : by have := s.high_le_size
+         exact s'.ge_elem arr[low]
+    := by
+  have h := s.ge_elem_low_of_sorted s_sorted nonempty
+  simp [Slice.ge_elem]
+  intro i in_bounds
+  simp [Slice.ge_elem] at h
+  have i_in_bounds : low ≤ i ∧ i < high := by omega
+  exact h i i_in_bounds
+
+/-- Two slices, `s₁` and `s₂`, remain less than or equal when we take the first
+element off of `s₂` and put it on the end of `s₁`.
+
+For example:
+```
+[1,2,3] ≤ [4,5,6]   is true, thus
+[1,2,3,4] ≤ [5,6]   is true as well
+```
+-/
+def Slice.le_of_swap_ends_le
+    {aux : Slice arr₁ low₁ high₁}
+    {arr : Slice arr₂ low₂ high₂}
+    (arr_sorted : arr.sorted)
+    (aux_le_arr : aux.le arr)
+    (high₁_lt_arr₁_size : high₁ < arr₁.size)
+    (low₂_lt_arr₂_size : low₂ < arr₂.size)
+    (arr₁'_def : arr₁' = arr₁.set ⟨high₁, high₁_lt_arr₁_size⟩ arr₂[low₂])
+    (s₁' : Slice arr₁' low₁ high₁.succ)
+    (s₂' : Slice arr₂ low₂.succ high₂)
+    (size_eq : arr₂.size = arr₁.size)
+    : s₁'.le s₂' := by
+  unfold Slice.le
+  intro i₁' i₂' i₂'_i₂'_in_range
+  unfold Nat.in_range at i₂'_i₂'_in_range
+  unfold Slice.le at aux_le_arr
+  by_cases h : i₁' = high₁
+  . simp [h, arr₁'_def]
+    rw [Slice.sorted] at arr_sorted
+    have low₂_lt_high₂ : low₂ < high₂ := by omega
+    have x := arr.ge_elem_low_succ_of_sorted arr_sorted low₂_lt_high₂ s₂'
+    simp [Slice.ge_elem] at x
+    have i₂'_in_range : low₂ + 1 ≤ ↑i₂' ∧ ↑i₂' < high₂ := by omega
+    have x2 := x i₂' i₂'_in_range
+    exact x2
+  . have i₁'_lt_arr₁_size : i₁'.val < arr₁.size := by omega
+    have i₂'_lt_arr₂_size : i₂'.val < arr₂.size := by omega
+    let i₁ : Fin arr₁.size := ⟨i₁', i₁'_lt_arr₁_size⟩
+    let i₂ : Fin arr₂.size := ⟨i₂', i₂'_lt_arr₂_size⟩
+    simp [arr₁'_def]
+    have high_ne_i₁' : high₁ ≠ i₁' := by omega
+    have i₁'_same := arr₁.get_set_ne
+      ⟨high₁, high₁_lt_arr₁_size⟩
+      arr₂[low₂]
+      i₁'_lt_arr₁_size
+      high_ne_i₁'
+    simp [i₁'_same]
+    have i₁_i₂_in_range : i₁.val.in_range low₁ high₁ ∧ i₂.val.in_range low₂ high₂ := by
+      simp [Nat.in_range]
+      omega
+    exact aux_le_arr i₁ i₂ i₁_i₂_in_range
+
+/--
+The elements at and following a pointer into a sorted slice are themselves
+sorted.
+-/
+def SlicePtrInclusive.sorted_of_right_sorted
+    (s : SlicePtrInclusive arr low high ptr)
+    (s_sorted : s.sorted)
+    : s.right.sorted := by
+  unfold Slice.sorted at *
+  intro i₁ i₂ adjacent_in_range
+  have adjacent_in_range' : i₁.val.adjacent_in_range i₂ low high := by
+    unfold Nat.adjacent_in_range at *
+    have := s.ptr_ge_low
+    omega
+  exact s_sorted i₁ i₂ adjacent_in_range'
+
+/--
+If `a` is greater or equal to all ements of a sorted slice `s`, then `s` remains sorted
+when `a` is appended on the right.
+-/
+def Slice.sorted_after_sorted_push
+    (s : Slice arr low high)
+    (s_sorted : s.sorted)
+    (high_lt_size : high < arr.size)
+    (arr'_def : arr' = arr.set ⟨high, high_lt_size⟩ a)
+    (s' : Slice arr' low high.succ)
+    (s_le_elem_a : s.le_elem a)
+    : s'.sorted := by
+  unfold Slice.sorted
+  intro i₁' i₂' adjacent_in_range'
+  simp [Nat.adjacent_in_range] at adjacent_in_range'
+  by_cases i₂'_eq_high : i₂' = high
+  . simp [i₂'_eq_high, arr'_def]
+    have i₁'_lt_arr_size : i₁'.val < arr.size := by omega
+    have high_ne_i₁' : high ≠ i₁' := by omega
+    have i₁'_same := arr.get_set_ne ⟨high, high_lt_size⟩ a i₁'_lt_arr_size high_ne_i₁'
+    rw [i₁'_same]
+    have in_bounds : i₁'.val.in_range low high := by simp [Nat.in_range]; omega
+    unfold Slice.le_elem at s_le_elem_a
+    exact s_le_elem_a i₁' in_bounds
+  . unfold Slice.sorted at s_sorted
+    have i₁'_lt_arr_size : i₁'.val < arr.size := by omega
+    have i₂'_lt_arr_size : i₂'.val < arr.size := by omega
+    simp [arr'_def]
+    have high_ne_i₁' : high ≠ i₁' := by omega
+    have high_ne_i₂' : high ≠ i₂' := by omega
+    have i₁'_same := arr.get_set_ne ⟨high, high_lt_size⟩ a i₁'_lt_arr_size high_ne_i₁'
+    have i₂'_same := arr.get_set_ne ⟨high, high_lt_size⟩ a i₂'_lt_arr_size high_ne_i₂'
+    simp [i₁'_same, i₂'_same]
+    let i₁ : Fin arr.size := ⟨i₁', i₁'_lt_arr_size⟩
+    let i₂ : Fin arr.size := ⟨i₂', i₂'_lt_arr_size⟩
+    have i₁_def : i₁ = ⟨i₁', i₁'_lt_arr_size⟩ := by rfl
+    have i₁_eq_i₁' : i₁' = i₁.val := by rw [i₁_def]
+    have adjacent_in_range : i₁.val.adjacent_in_range i₂ low high := by
+      simp [Nat.adjacent_in_range, i₂'_eq_high]
+      omega
+    exact s_sorted i₁ i₂ adjacent_in_range
